updated lean version to v4.6.0-rc1 for consistency with aeneas

test/lean/Proofs.lean
@@ -9,6 +9,8 @@ namespace test
 
 namespace arithmetics
 
+attribute [-simp] Bool.exists_bool
+
 def BigInt.valImpl (l : List U64) : Int :=
   match l with
   | a::b => a.val + (valImpl b) * (2 ^ 64)
@@ -20,7 +22,7 @@ lemma tmp : Inhabited U64 := by
   apply 0#u64
 
 -- Biggest part by Son Ho
-lemma BigInt.update_eq [Inhabited U64] (l : List U64) (i : Int) (x : U64)
+lemma BigInt.update_eq (l : List U64) (i : Int) (x : U64)
   (h0 : 0 ≤ i) (h1 : i < l.len) :
   BigInt.valImpl (l.update i x) = BigInt.valImpl l + (x - l.index i) * ((2 ^ 64) ^ i.toNat) := by
   match l with
@@ -29,7 +31,7 @@ lemma BigInt.update_eq [Inhabited U64] (l : List U64) (i : Int) (x : U64)
     simp at h1
     scalar_tac
   | h :: tl =>
-    simp at *
+    simp at h1
     if i = 0 then
       simp [*] -- By writing [*] I'm using the hypothesis i = 0
       unfold valImpl
@@ -37,17 +39,16 @@ lemma BigInt.update_eq [Inhabited U64] (l : List U64) (i : Int) (x : U64)
     else
       have hnz : i ≠ 0 := by scalar_tac
       -- This uses update_nzero_cons and index_nzero_cons
-      simp [*] -- By writing [*] I'm using the hypothesis i ≠ 0
+      simp only [h1, hnz, ne_eq, not_false_eq_true, List.update_nzero_cons, List.index_nzero_cons] -- By writing [*] I'm using the hypothesis i ≠ 0
       unfold valImpl
       -- Recursive call
       have heq := update_eq tl (i - 1) x (by scalar_tac) (by scalar_tac)
       rw [heq]
       rw [add_mul]
-      simp []
-      have hexpr (y : Int) : y * (2 ^ 64) ^ (Int.toNat i - 1) * 2 ^ 64 = y * (2 ^ 64) ^ Int.toNat i := by {
+      simp only [Int.pred_toNat]
+      have hexpr : ((2: Int) ^ 64) ^ (Int.toNat i - 1) * 2 ^ 64 = (2 ^ 64) ^ Int.toNat i := by {
         rw [←pow_mul]
-        rw [mul_assoc]
-        simp []
+        -- simp? []
         rw [←pow_add]
         rw [←pow_mul]
         rw [Nat.mul_sub_left_distrib]
@@ -56,76 +57,103 @@ lemma BigInt.update_eq [Inhabited U64] (l : List U64) (i : Int) (x : U64)
         have hgone : i ≥ 1 := by scalar_tac
         simp [hgone, *]
       }
+      simp only [mul_assoc]
       rw [hexpr]
       simp [add_assoc]
 
 
-lemma BigInt.len_spec
+@[simp] lemma BigInt.len_spec
   (N : Usize) (self : arithmetics.BigInt N) :
-  self.num.val.len = N.val := by
+  (self.num.val).len = N.val := by
   have h := self.num.property
   rw [List.len_eq_length]
   apply h
 
-def BigInt.val {N : Usize} [Inhabited U64] (x : BigInt N) : Int := valImpl x.num.val
+def BigInt.val {N : Usize} (x : BigInt N) : Int := valImpl x.num.val
 
 def BigInt.mod_value (N : Usize) : Int := (U64.max + 1) ^ (Int.toNat N.val)
 
 def BigInt.max_value (N : Usize) : Int := BigInt.mod_value N - 1
 
 theorem adc_for_add_with_carry_spec (a : U64) (b : U64) (carry : U8) :
-  ∃ new_carry, adc_for_add_with_carry a b carry = .ret new_carry ∧ 
-  new_carry = (a.val + b.val + carry.val) / (2 ^ 64) := by sorry
-
-theorem adc_for_add_with_carry_back_spec (a : U64) (b : U64) (carry : U8) :
-  ∃ new_a, adc_for_add_with_carry_back a b carry = .ret new_a ∧
-  new_a = (a.val + b.val + carry.val) % 2 ^ 64 := by sorry
+  ∃ new_carry r, adc_for_add_with_carry a b carry = .ret (new_carry, r) ∧ 
+  new_carry = (a.val + b.val + carry.val) / (2 ^ 64) ∧
+  r = (a.val + b.val + carry.val) % 2 ^ 64 := by sorry
 
 
 lemma add_with_carry_overflow [Inhabited U64] : 
   ∀ (N : Usize) (self : arithmetics.BigInt N) (other : arithmetics.BigInt N),
-  ∃ b, arithmetics.BigInt.add_with_carry N self other = .ret b ∧
+  ∃ b val, arithmetics.BigInt.add_with_carry N self other = .ret (b, val) ∧
   ¬b ↔ self.val + other.val ≤ BigInt.max_value N := sorry
-    -- by unfold arithmetics.BigInt.add_with_carry
+
+lemma BigInt.h_1_val (N: Usize) (bi : arithmetics.BigInt N) : N = 1#usize → BigInt.valImpl bi.num.val = (bi.num.val).index 0#usize.val  := 
+by {
+        simp [BigInt.val]; 
+        unfold BigInt.valImpl;
+        have h := BigInt.len_spec N bi;
+        -- intro
+        -- | ⟨w, bi.num.val = []⟩ => 
+
+        -- cases bi.num.val
+        -- . case nil hb => simp at h
+
+        match hq0 : bi.num.val with
+        | [] => simp [List.len_nil, Usize.ofInt_val_eq, hq0] at h; scalar_tac;
+        | hd :: tl => {
+          simp []
+          unfold BigInt.valImpl
+          match hq1 : tl with
+          | [] => simp [];
+          | hd::tl2 => simp [*, List.len_eq_length] at h; scalar_tac;
+        }
+      }
 
 -- Biggest part by Son Ho
-lemma add_with_carry_correct [Inhabited U64] :
+lemma add_with_carry_correct :
   ∀ (N : Usize) (self : arithmetics.BigInt N) (other : arithmetics.BigInt N),
-  ∃ v, arithmetics.BigInt.add_with_carry_back N self other = .ret v ∧
+  ∃ b v, arithmetics.BigInt.add_with_carry N self other = .ret (b, v) ∧
   v.val = (self.val + other.val) % (BigInt.mod_value N) := by
-    simp [arithmetics.BigInt.add_with_carry_back]
     intro N
+    intro self other
+    simp only [arithmetics.BigInt.add_with_carry]
     if hx : N = 1#usize then
-      rw [hx]
-      intro self other
-      simp 
-      progress with Array.index_usize_spec as ⟨ i, hi ⟩
+      simp only [hx, Usize.ofInt_val_eq]
+      simp only [Scalar.le_equiv, Scalar.ofInt_val_eq, le_refl, ↓reduceIte]
+      -- rw [hx]
+      progress with Array.index_mut_usize_spec as ⟨ i, hi, hid, hia ⟩
       progress with Array.index_usize_spec as ⟨ i0, hi0 ⟩
-      progress with adc_for_add_with_carry_back_spec as ⟨ i1, hi1 ⟩
+      progress with adc_for_add_with_carry_spec as ⟨ i1, hi1, hid1, hia1 ⟩
+      simp only [hia, hia1]
       progress with Array.update_usize_spec as ⟨ a1, ha1 ⟩
-      simp [BigInt.val, BigInt.max_value]
+      simp only [BigInt.val, BigInt.max_value]
       -- have h_self_val : i = self.val := by simp [hi, BigInt.val]; unfold BigInt.valImpl; simp [tmp, *]; unfold BigInt.valImpl; simp [tmp, *];
-      have h_bi_1_val : ∀ (bi : arithmetics.BigInt 1#usize), BigInt.valImpl bi.num.val = (bi.num.val).index 0#usize.val  := by intros; simp [hi, BigInt.val]; unfold BigInt.valImpl; sorry
       -- Proving that a1.val.len = 1 (remark: scalar_tac does it automatically)
       -- have h_array := a1.property
-      have h_valImpl := BigInt.update_eq self.num.val 0 i1 (by simp) (by scalar_tac)
-      simp [h_bi_1_val]
-      simp [ha1]
-      rw [h_valImpl]
-      simp
+      have h_valImpl := BigInt.update_eq self.num.val 0 hi1 (by simp) (by scalar_tac)
+
+      -- simp [hx] at self
+      -- simp [hx] at other
+      rw [BigInt.h_1_val]
+      simp only [BigInt.h_1_val, hx]
+      exists i1 != 0#u8, { num := a1 }
+      simp only [and_self, Scalar.ofInt_val_eq, le_refl, BigInt.len_spec, zero_lt_one,
+        List.index_update_eq, add_zero, Int.reducePow, true_and]
+      simp only [ha1]
+      simp only [Scalar.ofInt_val_eq, le_refl]
       -- Because length = 1
-      have hself : BigInt.valImpl self.num.val = (self.num.val.index 0).val := by unfold BigInt.valImpl; sorry
-      rw [hself]
+      -- have hself : BigInt.valImpl self.num.val = (self.num.val.index 0).val := by unfold BigInt.valImpl; sorry
+      -- rw [hself]
       
-      rw [hi1]
+      simp [List.index_update_eq, hx, BigInt.len_spec]
+      rw [hia1]
       
-      have h64 : BigInt.mod_value 1#usize = 2 ^ 64 := by unfold BigInt.mod_value; simp []
+      have h64 : BigInt.mod_value 1#usize = 2 ^ 64 := by unfold BigInt.mod_value; simp [U64.max]
       rw [h64]
       -- Finishing the proof
       rw [hi0]
-      simp
-      rw [hi]
-      simp
+      rw [hid]
+      simp only [Scalar.ofInt_val_eq, add_zero]
+      simp only [hx]
     else
       sorry
 
